games/Sets.v
@@ -1,0 +1,81 @@
+Require Import LogicalRelations.
+
+Notation set U := (U -> Prop).
+
+Definition subset {U} : relation (set U) :=
+  - ==> impl.
+
+Definition set_rel {A B} (R : rel A B) : rel (set A) (set B) :=
+  set_le R /\ set_ge R.
+
+Definition set_union {U} (s : set (set U)) : set U :=
+  fun x => exists sx, s sx /\ sx x.
+
+Lemma set_union_ub {U} (s : set (set U)) (sx : set U) :
+  s sx -> subset sx (set_union s).
+Proof.
+  firstorder.
+Qed.
+
+Lemma set_union_lub {U} (s : set (set U)) (sy : set U) :
+  (forall sx, s sx -> subset sx sy) ->
+  subset (set_union s) sy.
+Proof.
+  firstorder.
+Qed.
+
+Definition set_inter {U} (s : set (set U)) : set U :=
+  fun x => forall sx, s sx -> sx x.
+
+Inductive set_map {A B} (f : A -> B) (sA : set A) : set B :=
+  set_map_intro a :
+    sA a -> set_map f sA (f a).
+
+Hint Constructors set_map.
+
+Global Instance set_map_le :
+  Monotonic
+    (@set_map)
+    (forallr RA, forallr RB, (RA ++> RB) ++> set_le RA ++> set_le RB).
+Proof.
+  intros A1 A2 RA B1 B2 RB f g Hfg sA1 sA2 HsA b1 Hb1.
+  destruct Hb1 as [a1]. edestruct HsA as (a2 & Ha2 & Ha); eauto.
+Qed.
+
+Inductive set_bind {A B} (f : A -> set B) (sa: set A) : set B :=
+  set_bind_intro a b :
+    sa a -> f a b -> set_bind f sa b.
+
+Hint Constructors set_bind.
+
+Global Instance set_bind_le :
+  Monotonic
+    (@set_bind)
+    (forallr RA, forallr RB, (RA ++> set_le RB) ++> set_le RA ++> set_le RB).
+Proof.
+  intros A1 A2 RA B1 B2 RB f g Hfg sa sb Hs.
+  intros _ [a1 b1 Ha1 Hb1].
+  edestruct Hs as (a2 & Ha2 & Ha); eauto.
+  edestruct Hfg as (b2 & Hb2 & Hb); eauto.
+Qed.
+
+Definition set_bind_all {A B} (f : A -> set B) (sA : set A) : set B :=
+  set_union (set_map f sA).
+
+Definition set_bind_ex {A B} (f : A -> set B) (sA : set A) : set B :=
+  set_inter (set_map f sA).
+
+(** This definition is identical to [eq]. *)
+
+Inductive singl {A} (a : A) : set A :=
+  singl_intro : singl a a.
+
+Hint Constructors singl.
+
+Global Instance eq_le :
+  Monotonic (@singl) (forallr R, R ++> set_le R).
+Proof.
+  intros A B R a b Hab _ [ ]. eauto.
+Qed.
+
+
